Notes based on \citet{craig2018course} and on the Partial Differential Equations
course ministered by Emanuel Carneiro on 2011 at IMPA.

\section{The Wave Equation}

\subsection{d'Alembert formula}

Consider the following problem:
\begin{align*}
  &\partial_t^2 u - \partial^2_x u = 0,\\
  & u(0,x) = f(x), \quad \partial_t u(0,x) = g(x).
\end{align*}

To solve this, we'll use a change of coordinates 
\begin{displaymath}
  r := x + t, \quad s:= x -t. 
\end{displaymath}

Now, let's apply the Chain rule for $g(r,s) = (\frac{r-s}{2},\frac{r+s}{2})$,
\begin{align*}
  (\partial_r v, \partial_s v) = D(u\circ g)(r,s) = D u(t,x) D g(r,s)
  &= (\partial_t u, \partial_x u)
  \begin{pmatrix}
    \partial_r g_1 & \partial_s g_1 \\
    \partial_r g_2 & \partial_s g_2
  \end{pmatrix}\\
  &= (\partial_t u, \partial_x u)
  \begin{pmatrix}
    1/2 & -1/2 \\
    1/2 & 1/2 
  \end{pmatrix}\\
  &=
  \left(\frac{\partial_t u + \partial_x y}{2}, 
  \frac{\partial_t u - \partial_x y}{2}\right).
\end{align*}
Which implies that $\partial_r = $




